Change execution to flatter relation structure (Part 5)

src/ReactorModel/Execution/Theorems/Step/Apply.lean
@@ -1,6 +1,7 @@
 import ReactorModel.Execution.Basic
 import ReactorModel.Execution.Theorems.State
 
+noncomputable section
 open Classical ReactorType Execution State
 
 namespace Execution.Step.Apply
@@ -24,41 +25,66 @@ theorem preserves_unchanged (e : s₁ -[c]→ s₂) (h : ¬c.Targets cpt i) :
   cases e <;> try exact .refl _
   all_goals simp [LawfulUpdate.obj?_preserved (Change.Targets.norm_not h) ‹_›]
 
-theorem ne_target_comm {c₁ c₂ : Change} 
-    (ht : c₁.target ≠ c₂.target ∨ c₁.target = none) (e₁ : s -[c₁]→ s₁) (e₁₂ : s₁ -[c₂]→ s₁₂) 
-    (e₂ : s -[c₂]→ s₂) (e₂₁ : s₂ -[c₁]→ s₂₁) : s₁₂ = s₂₁ := by
-  /-ext1 <;> cases_change c₁ <;> cases_change c₂ <;> simp [apply, Change.target] at *
-  all_goals 
-    try rfl
-    try exact LawfulUpdatable.update_ne_comm $ by simp_all
-  apply Partial.update_ne_comm _ ht
-  -/
-  sorry
+theorem events_congr (e : s₁ -[c]→ s₂) (e' : s₁' -[c]→ s₂') (he : s₁.events = s₁'.events) : 
+    s₂.events = s₂'.events := by 
+  cases e <;> cases e' <;> simp [he]
+  exact schedule_events_congr he
+
+end Execution.Step.Apply
+
+namespace Execution.Step.Apply
+
+variable [Readable α] {s s₁ s₂ : State α} {c : Change}
 
 theorem rtr_congr (e : s₁ -[c]→ s₂) (e' : s₁' -[c]→ s₂') 
     (h : s₁.rtr = s₁'.rtr) : s₂.rtr = s₂'.rtr := by 
-  sorry
-
-theorem events_congr (e : s₁ -[c]→ s₂) (e' : s₁' -[c]→ s₂') 
-    (hr : s₁.rtr = s₁'.rtr) (he : s₁.events = s₁'.events) : s₂.events = s₂'.events := by 
-  sorry
+  cases e <;> cases e' <;> simp [State.schedule_preserves_rtr, h]
+  all_goals rw [h] at *; exact LawfulUpdate.unique ‹_› ‹_›  
 
 theorem comm_record (e₁ : s -[c]→ s₁) (e₂ : (s.record rcn) -[c]→ s₂) : s₁.record rcn = s₂ := by
   ext1
   case rtr      => exact e₁.rtr_congr e₂ (s.record_preserves_rtr rcn)
   case tag      => simp [record_preserves_tag, ←e₁.preserves_tag, ←e₂.preserves_tag]
   case progress => simp [record_progress_eq, ←e₂.preserves_progress, e₁.preserves_progress]
-  case events   => exact e₁.events_congr e₂ (s.record_preserves_rtr rcn) (s.record_preserves_events rcn)
+  case events   => exact e₁.events_congr e₂ (s.record_preserves_events rcn)
+
+theorem deterministic (e₁ : s -[c]→ s₁) (e₂ : s -[c]→ s₂) : s₁ = s₂ := by
+  cases e₁ <;> cases e₂ <;> simp <;> exact LawfulUpdate.unique ‹_› ‹_›
 
 end Execution.Step.Apply
 
-theorem Execution.Step.Apply.deterministic [Readable α] {s s₁ s₂ : State α} {c : Change} 
-    (e₁ : s -[c]→ s₁) (e₂ : s -[c]→ s₂) : s₁ = s₂ := by
-  cases e₁ <;> cases e₂ <;> simp <;> exact LawfulUpdate.unique ‹_› ‹_›
+namespace Execution.Step.Apply
+
+variable [Proper α] {c₁ c₂ : Change} {s s₁ s₂ s₁₂ s₂₁ : State α}
+
+theorem ne_target_comm (ht : c₁.target ≠ c₂.target ∨ c₁.target = none) (e₁ : s -[c₁]→ s₁) 
+    (e₁₂ : s₁ -[c₂]→ s₁₂) (e₂ : s -[c₂]→ s₂) (e₂₁ : s₂ -[c₁]→ s₂₁) : s₁₂ = s₂₁ := by
+  cases e₁ <;> cases e₁₂ <;> cases e₂ <;> cases e₂₁ <;> simp [Change.target] at ht ⊢ 
+  case act.act.act.act =>               exact schedule_ne_comm ht
+  case inp.act.act.inp u₁ _ _ _ _ u₂ => simp [schedule_preserves_rtr] at u₂; cases LawfulUpdate.unique u₁ u₂; rfl
+  case out.act.act.out u₁ _ _ _ _ u₂ => simp [schedule_preserves_rtr] at u₂; cases LawfulUpdate.unique u₁ u₂; rfl
+  case stv.act.act.stv u₁ _ _ _ _ u₂ => simp [schedule_preserves_rtr] at u₂; cases LawfulUpdate.unique u₁ u₂; rfl
+  case act.inp.inp.act u₁ _ u₂ =>       simp [schedule_preserves_rtr] at u₂; cases LawfulUpdate.unique u₁ u₂; rfl
+  case act.out.out.act u₁ _ u₂ =>       simp [schedule_preserves_rtr] at u₂; cases LawfulUpdate.unique u₁ u₂; rfl
+  case act.stv.stv.act u₁ _ u₂ =>       simp [schedule_preserves_rtr] at u₂; cases LawfulUpdate.unique u₁ u₂; rfl
+  all_goals
+    try exact LawfulUpdate.unique ‹_› ‹_›  
+    try case _ u₁ _ _ _ u₂ _ u₃ _ u₄ => exact LawfulUpdate.ne_comm u₁ u₂ u₃ u₄ $ by simp [ht]
+
+-- TODO: Formalize this a bit nicer. Add an `apply` function to `State` when `Proper α`.
+open Updatable in
+def construct (s : State α) : (c : Change) → (s' : State α) × (s -[c]→ s')
+  | .inp i v   => ⟨{ s with rtr := update s.rtr .inp i v }, inp $ LawfulUpdatable.lawful ..⟩ 
+  | .out i v   => ⟨{ s with rtr := update s.rtr .out i v }, out $ LawfulUpdatable.lawful ..⟩ 
+  | .stv i v   => ⟨{ s with rtr := update s.rtr .stv i v }, stv $ LawfulUpdatable.lawful ..⟩ 
+  | .act i t v => ⟨s.schedule i t v, act⟩  
+  | .mut _     => ⟨s, «mut»⟩
+
+end Execution.Step.Apply
 
 namespace Execution.Step.Apply.RTC
 
-variable [Indexable α] {s₁ : State α} {c : Change} {out out₁ out₂ : Reaction.Output}
+variable [Indexable α] {s₁ : State α} {out : Reaction.Output}
 
 theorem preserves_tag (e : s₁ -[out]→ s₂) : s₁.tag = s₂.tag := by 
   induction e
@@ -83,20 +109,42 @@ theorem preserves_unchanged {cpt : Component.Valued}
     have ⟨hh, ht⟩ := List.all₂_cons _ _ _ |>.mp h
     exact e.preserves_unchanged hh ▸ hi ht 
 
+end Execution.Step.Apply.RTC
+
+namespace Execution.Step.Apply.RTC
+
+variable [Readable α] {s s₁ s₂ : State α} {out : Reaction.Output} 
+
+theorem comm_record (e₁ : s -[out]→ s₁) (e₂ : (s.record rcn) -[out]→ s₂) : s₁.record rcn = s₂ := by
+  induction e₁ <;> cases e₂
+  case refl.refl => rfl
+  case trans.trans e₁ _ hi _ e₂ e₂' => exact hi $ (e₁.comm_record e₂).symm ▸ e₂'
+
+theorem deterministic (e₁ : s -[out]→ s₁) (e₂ : s -[out]→ s₂) : s₁ = s₂ := by
+  induction e₁ generalizing s₂ <;> cases e₂
+  case refl.refl => rfl
+  case trans.trans e₁ _ hi _ e₂ e₂' => exact hi $ (e₁.deterministic e₂) ▸ e₂'
+
+end Execution.Step.Apply.RTC
+
+namespace Execution.Step.Apply.RTC
+
+variable [Proper α] {s s₁ s₂ : State α} {c : Change} {out out₁ out₂ : Reaction.Output} 
+
 theorem ne_targets_comm_apply 
     (ht : ∀ {t}, c.target = some t → t ∉ out.targets) (eₒ : s -[out]→ sₒ) (eₒ₁ : sₒ -[c]→ sₒ₁) 
     (e₁ : s -[c]→ s₁) (e₁ₒ : s₁ -[out]→ s₁ₒ) : sₒ₁ = s₁ₒ := by
-  /-
-  induction out generalizing s <;> simp [apply'] at *
-  case cons hd tl hi =>
+  induction eₒ generalizing s₁ <;> cases e₁ₒ
+  case refl.refl => exact eₒ₁.deterministic e₁
+  case trans.trans hd _ s' tl _ eₒ _ hi _ e₁ₒ e₁ₒ' =>
     suffices h : hd.target ≠ c.target ∨ hd.target = none by 
-      rw [hi $ fun _ _ h hm => ht _ _ h $ List.mem_targets_cons hm, apply_ne_target_comm h]
+      have ⟨_, e'⟩ := Apply.construct s' c
+      cases Apply.ne_target_comm h eₒ e' e₁ e₁ₒ
+      exact hi (ht · $ Reaction.Output.mem_targets_cons ·) ‹_› ‹_› ‹_›
     by_contra hc
     push_neg at hc
     have ⟨_, h⟩ := Option.ne_none_iff_exists.mp hc.right
-    exact ht _ _ (hc.left ▸ h.symm) $ List.target_mem_targets (by simp) h.symm
-  -/
-  sorry
+    exact ht (hc.left ▸ h.symm) $ Reaction.Output.target_mem_targets (by simp) h.symm
 
 theorem disjoint_targets_comm 
     (ht : Disjoint out₁.targets out₂.targets) (e₁ : s -[out₁]→ s₁) (e₁₂ : s₁ -[out₂]→ s₁₂) 
@@ -125,16 +173,4 @@ theorem disjoint_targets_comm
   -/
   sorry
 
-theorem comm_record (e₁ : s -[out]→ s₁) (e₂ : (s.record rcn) -[out]→ s₂) : s₁.record rcn = s₂ := by
-  induction e₁ <;> cases e₂
-  case refl.refl => rfl
-  case trans.trans e₁ _ hi _ e₂ e₂' => exact hi $ (e₁.comm_record e₂).symm ▸ e₂'
-
 end Execution.Step.Apply.RTC
-
-theorem Execution.Step.Apply.RTC.deterministic 
-    [Readable α] {s s₁ s₂ : State α} {out : Reaction.Output} 
-    (e₁ : s -[out]→ s₁) (e₂ : s -[out]→ s₂) : s₁ = s₂ := by
-  induction e₁ generalizing s₂ <;> cases e₂
-  case refl.refl => rfl
-  case trans.trans e₁ _ hi _ e₂ e₂' => exact hi $ (e₁.deterministic e₂) ▸ e₂'
